Some work on the translator.

translator/ml_translatorScript.sml
@@ -1,8 +1,7 @@
 open HolKernel Parse boolLib bossLib;
 val _ = new_theory "ml_translator";
-open astTheory libTheory altBigStepTheory semanticPrimitivesTheory;
-open terminationTheory;
-open bigBigEquivTheory;
+open astTheory libTheory semanticPrimitivesTheory bigStepTheory;
+open terminationTheory bigClockTheory;
 open arithmeticTheory listTheory combinTheory pairTheory;
 open integerTheory;
 open lcsymtacs;
@@ -14,12 +13,12 @@ infix \\ val op \\ = op THEN;
 
 val Eval_def = Define `
   Eval env exp P =
-    ?res. evaluate' empty_store env exp (empty_store,Rval res) /\ P (res:v)`;
+    ?res. evaluate F env (0,empty_store) exp ((0,empty_store),Rval res) /\ P (res:v)`;
 
 val evaluate_closure_def = Define `
   evaluate_closure input cl output =
-    ?env exp. (do_app empty_store ARB Opapp cl input = SOME (empty_store,env,exp)) /\
-              evaluate' empty_store env exp (empty_store,Rval (output))`;
+    ?env exp. (do_app ARB empty_store Opapp cl input = SOME (env,empty_store,exp)) /\
+              evaluate F env (0,empty_store) exp ((0,empty_store),Rval (output))`;
 
 val AppReturns_def = Define ` (* think of this as a Hoare triple {P} cl {Q} *)
   AppReturns P cl Q =
@@ -62,27 +61,10 @@ val PreImp_def = Define `
 
 (* Theorems *)
 
-val big_exp_determ' = store_thm("big_exp_determ'",
- ``(!s env e r1.
-      evaluate' s env e r1 ==>
-     !r2. evaluate' s env e r2 ==> (r1 = r2)) /\
-   (!s env es r1.
-      evaluate_list' s env es r1 ==>
-      !r2. evaluate_list' s env es r2 ==> (r1 = r2)) /\
-   (!s env v pes errv r1.
-      evaluate_match' s env v pes errv r1 ==>
-      !r2. evaluate_match' s env v pes errv r2 ==> (r1 = r2))``,
-  HO_MATCH_MP_TAC evaluate'_ind >> rw [] >>
-  pop_assum (ASSUME_TAC o SIMP_RULE (srw_ss ()) [Once evaluate'_cases]) >>
-  fs [] >> rw [] >> fs [] >> res_tac >> fs [] >> rw [] >>
-  res_tac >> fs [] >> metis_tac []);
-
-val evaluate_cases = evaluate'_cases;
-
 val evaluate_11_Rval = store_thm("evaluate_11_Rval",
-  ``evaluate' s env exp (s1,Rval res1) ==>
-    evaluate' s env exp (s2,Rval res2) ==> (res1 = res2)``,
-  REPEAT STRIP_TAC \\ IMP_RES_TAC big_exp_determ'
+  ``evaluate b env s exp (s1,Rval res1) ==>
+    evaluate b env s exp (s2,Rval res2) ==> (res1 = res2)``,
+  REPEAT STRIP_TAC \\ IMP_RES_TAC big_exp_determ
   \\ FULL_SIMP_TAC (srw_ss()) []);
 
 val Eval_Arrow = store_thm("Eval_Arrow",
@@ -100,16 +82,16 @@ val Eval_Arrow = store_thm("Eval_Arrow",
   \\ METIS_TAC []);
 
 val Eval_Fun = store_thm("Eval_Fun",
-  ``(!v x. a x v ==> Eval ((name,v)::env) body (b ((f:'a->'b) x))) ==>
-    Eval env (Fun name body) ((a --> b) f)``,
+  ``(!v x. a x v ==> Eval (menv,cenv,(name,v)::env) body (b ((f:'a->'b) x))) ==>
+    Eval (menv,cenv,env) (Fun name body) ((a --> b) f)``,
   SIMP_TAC std_ss [Eval_def,Arrow_def] \\ REPEAT STRIP_TAC
   \\ ONCE_REWRITE_TAC [evaluate_cases] \\ SIMP_TAC (srw_ss()) []
   \\ ASM_SIMP_TAC (srw_ss()) [AppReturns_def,Eval_def,do_app_def,
        bind_def,evaluate_closure_def]);
 
 val Eval_Fun_Eq = store_thm("Eval_Fun_Eq",
-  ``(!v. a x v ==> Eval ((name,v)::env) body (b (f x))) ==>
-    Eval env (Fun name body) ((Eq a x --> b) f)``,
+  ``(!v. a x v ==> Eval (menv,cenv,(name,v)::env) body (b (f x))) ==>
+    Eval (menv,cenv,env) (Fun name body) ((Eq a x --> b) f)``,
   SIMP_TAC std_ss [Eval_def,Arrow_def] \\ REPEAT STRIP_TAC
   \\ ONCE_REWRITE_TAC [evaluate_cases] \\ SIMP_TAC (srw_ss()) []
   \\ ASM_SIMP_TAC (srw_ss()) [AppReturns_def,evaluate_closure_def,
@@ -125,41 +107,42 @@ val Eq_IMP_And = store_thm("Eq_IMP_And",
   ``(!x. P x ==> Eval env (Fun name exp) ((Eq a x --> b) f)) ==>
     Eval env (Fun name exp) ((And a P --> b) f)``,
   FULL_SIMP_TAC std_ss [Eval_def,Arrow_def,AppReturns_def,And_def,Eq_def]
-  \\ ONCE_REWRITE_TAC [evaluate'_cases] \\ SIMP_TAC (srw_ss()) []);
+  \\ ONCE_REWRITE_TAC [evaluate_cases] \\ SIMP_TAC (srw_ss()) []);
 
 val Eval_Fun_And = store_thm("Eval_Fun_And",
-  ``(!v x. P x ==> a x v ==> Eval ((name,v)::env) body (b (f x))) ==>
-    Eval env (Fun name body) ((And a P --> b) f)``,
+  ``(!v x. P x ==> a x v ==> Eval (menv,cenv,(name,v)::env) body (b (f x))) ==>
+    Eval (menv,cenv,env) (Fun name body) ((And a P --> b) f)``,
   FULL_SIMP_TAC std_ss [GSYM And_def,AND_IMP_INTRO]
   \\ REPEAT STRIP_TAC \\ MATCH_MP_TAC Eval_Fun \\ ASM_SIMP_TAC std_ss []);
 
 val Eval_Let = store_thm("Eval_Let",
-  ``Eval env exp (a res) /\
-    (!v. a res v ==> Eval ((name,v)::env) body (b (f res))) ==>
-    Eval env (Let name exp body) (b (LET f res))``,
+  ``Eval (menv,cenv,env) exp (a res) /\
+    (!v. a res v ==> Eval (menv,cenv,(name,v)::env) body (b (f res))) ==>
+    Eval (menv,cenv,env) (Let name exp body) (b (LET f res))``,
   SIMP_TAC std_ss [Eval_def,Arrow_def] \\ REPEAT STRIP_TAC
   \\ ONCE_REWRITE_TAC [evaluate_cases] \\ SIMP_TAC (srw_ss()) []
   \\ RES_TAC \\ Q.EXISTS_TAC `res''` \\ FULL_SIMP_TAC std_ss [LET_DEF,bind_def]
-  \\ Q.LIST_EXISTS_TAC [`res'`,`empty_store`] \\ FULL_SIMP_TAC std_ss []);
+  \\ Q.LIST_EXISTS_TAC [`res'`,`0,empty_store`] \\ FULL_SIMP_TAC std_ss []);
 
 val Eval_Var_SWAP_ENV = store_thm("Eval_Var_SWAP_ENV",
-  ``!env1.
-      Eval env1 (Var (Short name)) P /\ (lookup name env = lookup name env1) ==>
-      Eval env (Var (Short name)) P``,
-  SIMP_TAC (srw_ss()) [Once evaluate_cases,Eval_def]
-  \\ SIMP_TAC (srw_ss()) [Once evaluate_cases,Eval_def]);
+  ``!menv1 cenv1 env1.
+      Eval (menv1,cenv1,env1) (Var (Short name)) P /\ (lookup name env = lookup name env1) ==>
+      Eval (menv,cenv,env) (Var (Short name)) P``,
+  SIMP_TAC (srw_ss()) [Once evaluate_cases,Eval_def, lookup_var_id_def]
+  \\ SIMP_TAC (srw_ss()) [Once evaluate_cases,Eval_def, lookup_var_id_def]);
 
 val LOOKUP_VAR_def = Define `
-  LOOKUP_VAR name env x = (lookup name env = SOME x)`;
+  LOOKUP_VAR name (menv,cenv,env) x = (lookup name env = SOME x)`;
 
 val LOOKUP_VAR_THM = store_thm("LOOKUP_VAR_THM",
   ``LOOKUP_VAR name env x ==> Eval env (Var (Short name)) ($= x)``,
-  SIMP_TAC (srw_ss()) [Once evaluate_cases,Eval_def,LOOKUP_VAR_def]);
+  PairCases_on `env` >>
+  SIMP_TAC (srw_ss()) [Once evaluate_cases,Eval_def,LOOKUP_VAR_def, lookup_var_id_def]);
 
 val LOOKUP_VAR_SIMP = store_thm("LOOKUP_VAR_SIMP",
-  ``LOOKUP_VAR name ((x,v)::env) y =
-    if x = name then (v = y) else LOOKUP_VAR name env y``,
-  SIMP_TAC std_ss [LOOKUP_VAR_def,lookup_def] \\ SRW_TAC [] []);
+  ``LOOKUP_VAR name (menv,cenv,(x,v)::env) y =
+    if x = name then (v = y) else LOOKUP_VAR name (menv,cenv,env) y``,
+  SIMP_TAC std_ss [LOOKUP_VAR_def,lookup_def, lookup_var_id_def] \\ SRW_TAC [] []);
 
 val Eval_Val_INT = store_thm("Eval_Val_INT",
   ``!n. Eval env (Lit (IntLit n)) (INT n)``,
@@ -186,7 +169,7 @@ val Eval_Or = store_thm("Eval_Or",
   \\ ONCE_REWRITE_TAC [evaluate_cases] \\ SIMP_TAC (srw_ss()) []
   \\ Q.EXISTS_TAC `(Litv (Bool b1))` \\ Cases_on `b1`
   \\ FULL_SIMP_TAC (srw_ss()) [do_log_def]
-  \\ Q.EXISTS_TAC `empty_store` \\ FULL_SIMP_TAC std_ss []
+  \\ Q.EXISTS_TAC `0,empty_store` \\ FULL_SIMP_TAC std_ss []
   \\ ONCE_REWRITE_TAC [evaluate_cases] \\ SIMP_TAC (srw_ss()) []);
 
 val Eval_And = store_thm("Eval_And",
@@ -198,7 +181,7 @@ val Eval_And = store_thm("Eval_And",
   \\ ONCE_REWRITE_TAC [evaluate_cases] \\ SIMP_TAC (srw_ss()) []
   \\ Q.EXISTS_TAC `(Litv (Bool b1))` \\ Cases_on `b1`
   \\ FULL_SIMP_TAC (srw_ss()) [do_log_def]
-  \\ Q.EXISTS_TAC `empty_store` \\ FULL_SIMP_TAC std_ss []
+  \\ Q.EXISTS_TAC `0,empty_store` \\ FULL_SIMP_TAC std_ss []
   \\ ONCE_REWRITE_TAC [evaluate_cases] \\ SIMP_TAC (srw_ss()) []);
 
 val Eval_If = store_thm("Eval_If",
@@ -213,10 +196,10 @@ val Eval_If = store_thm("Eval_If",
   \\ Cases_on `b1` \\ FULL_SIMP_TAC std_ss []
   THEN1 (Q.EXISTS_TAC `res` \\ ASM_SIMP_TAC std_ss []
     \\ Q.EXISTS_TAC `Litv (Bool T)` \\ ASM_SIMP_TAC (srw_ss()) [do_if_def]
-    \\ Q.EXISTS_TAC `empty_store` \\ FULL_SIMP_TAC std_ss [])
+    \\ Q.EXISTS_TAC `0,empty_store` \\ FULL_SIMP_TAC std_ss [])
   THEN1 (Q.EXISTS_TAC `res` \\ ASM_SIMP_TAC std_ss []
     \\ Q.EXISTS_TAC `Litv (Bool F)` \\ ASM_SIMP_TAC (srw_ss()) [do_if_def]
-    \\ Q.EXISTS_TAC `empty_store` \\ FULL_SIMP_TAC std_ss []));
+    \\ Q.EXISTS_TAC `0,empty_store` \\ FULL_SIMP_TAC std_ss []));
 
 val Eval_Bool_Not = store_thm("Eval_Bool_Not",
   ``Eval env x1 (BOOL b1) ==>
@@ -226,7 +209,7 @@ val Eval_Bool_Not = store_thm("Eval_Bool_Not",
   \\ ONCE_REWRITE_TAC [evaluate_cases] \\ SIMP_TAC (srw_ss()) []
   \\ FULL_SIMP_TAC (srw_ss()) [bigClockTheory.do_app_cases]
   \\ Q.LIST_EXISTS_TAC [`(Litv (Bool b1))`, `Litv (Bool F)`, `Lit (Bool ~b1)`,
-                        `empty_store`, `empty_store`]
+                        `0,empty_store`, `empty_store`]
   \\ FULL_SIMP_TAC std_ss []
   \\ ONCE_REWRITE_TAC [evaluate_cases] \\ SIMP_TAC (srw_ss()) []
   \\ SIMP_TAC (srw_ss ()) [do_eq_def]);
@@ -240,15 +223,15 @@ val Eval_Implies = store_thm("Eval_Implies",
   \\ ONCE_REWRITE_TAC [evaluate_cases] \\ SIMP_TAC (srw_ss()) []
   \\ Q.EXISTS_TAC `(Litv (Bool b1))` \\ Cases_on `b1`
   \\ FULL_SIMP_TAC (srw_ss()) [do_if_def]
-  \\ Q.EXISTS_TAC `empty_store` \\ FULL_SIMP_TAC std_ss []
+  \\ Q.EXISTS_TAC `0,empty_store` \\ FULL_SIMP_TAC std_ss []
   \\ ONCE_REWRITE_TAC [evaluate_cases] \\ SIMP_TAC (srw_ss()) []);
 
 val Eval_Var_SIMP = store_thm("Eval_Var_SIMP",
-  ``Eval ((x,v)::env) (Var (Short y)) p =
-      if x = y then p v else Eval env (Var (Short y)) p``,
-  SIMP_TAC (srw_ss()) [Eval_def,Once evaluate_cases,lookup_def]
+  ``Eval (menv,cenv,(x,v)::env) (Var (Short y)) p =
+      if x = y then p v else Eval (menv,cenv,env) (Var (Short y)) p``,
+  SIMP_TAC (srw_ss()) [Eval_def,Once evaluate_cases,lookup_def, lookup_var_id_def]
   \\ SRW_TAC [] [] \\ SIMP_TAC (srw_ss()) [Eval_def,Once evaluate_cases,
-       lookup_def]);
+       lookup_def, lookup_var_id_def]);
 
 val Eval_Eq = store_thm("Eval_Eq",
   ``Eval env exp (a x) ==> Eval env exp ((Eq a x) x)``,
@@ -265,7 +248,7 @@ val Eval_FUN_FORALL = store_thm("Eval_FUN_FORALL",
     Eval env exp ((FUN_FORALL x. p x) f)``,
   SIMP_TAC std_ss [Eval_def,Arrow_def,Eq_def] \\ REPEAT STRIP_TAC
   \\ FULL_SIMP_TAC std_ss [AppReturns_def,FUN_FORALL]
-  \\ `?res. evaluate' empty_store env exp (empty_store,Rval res)` by METIS_TAC []
+  \\ `?res. evaluate F env (0,empty_store) exp ((0,empty_store),Rval res)` by METIS_TAC []
   \\ Q.EXISTS_TAC `res` \\ FULL_SIMP_TAC std_ss []
   \\ REPEAT STRIP_TAC \\ Q.PAT_ASSUM `!x.bbb` (STRIP_ASSUME_TAC o Q.SPEC `y`)
   \\ IMP_RES_TAC evaluate_11_Rval \\ FULL_SIMP_TAC (srw_ss()) []);
@@ -287,7 +270,7 @@ val FUN_FORALL_PUSH1 = prove(
   THEN1 METIS_TAC [evaluate_11_Rval]
   \\ REPEAT STRIP_TAC
   \\ FULL_SIMP_TAC std_ss [PULL_FORALL] \\ RES_TAC
-  \\ POP_ASSUM (fn th => STRIP_ASSUME_TAC (Q.SPEC `ARB` th) THEN ASSUME_TAC th)
+  \\ POP_ASSUM (fn th => STRIP_ASSUME_TAC (Q.SPEC `env` th) THEN ASSUME_TAC th)
   \\ FULL_SIMP_TAC std_ss []
   \\ Q.EXISTS_TAC `u` \\ FULL_SIMP_TAC std_ss []
   \\ REPEAT STRIP_TAC
@@ -310,15 +293,15 @@ val FUN_QUANT_SIMP = save_thm("FUN_QUANT_SIMP",
 val Eval_Recclosure_ALT = store_thm("Eval_Recclosure_ALT",
   ``!funs fname name body.
     (!v. a n v ==>
-  Eval ((name,v)::FOLDR (\(f,x,e) env'. (f,Recclosure env2 funs f)::env') env2
-           funs) body (b (f n))) ==>
-    LOOKUP_VAR fname env (Recclosure env2 funs fname) ==>
+  Eval (menv2,cenv2, ((name,v)::FOLDR (\(f,x,e) env'. (f,Recclosure (menv2,cenv2,env2) funs f)::env') env2
+           funs)) body (b (f n))) ==>
+    LOOKUP_VAR fname env (Recclosure (menv2,cenv2,env2) funs fname) ==>
     (find_recfun fname funs = SOME (name,body)) ==>
     Eval env (Var (Short fname)) ((Eq a n --> b) f)``,
   NTAC 6 STRIP_TAC \\ IMP_RES_TAC LOOKUP_VAR_THM
   \\ POP_ASSUM MP_TAC \\ POP_ASSUM (K ALL_TAC) \\ POP_ASSUM MP_TAC
   \\ FULL_SIMP_TAC std_ss [Eval_def,Arrow_def] \\ REPEAT STRIP_TAC
-  \\ POP_ASSUM MP_TAC \\ POP_ASSUM MP_TAC \\ ONCE_REWRITE_TAC [evaluate'_cases]
+  \\ POP_ASSUM MP_TAC \\ POP_ASSUM MP_TAC \\ ONCE_REWRITE_TAC [evaluate_cases]
   \\ FULL_SIMP_TAC (srw_ss()) [AppReturns_def,Eq_def,
        do_app_def,evaluate_closure_def]
   \\ REPEAT STRIP_TAC \\ FULL_SIMP_TAC (srw_ss()) []
@@ -326,8 +309,8 @@ val Eval_Recclosure_ALT = store_thm("Eval_Recclosure_ALT",
 
 val Eval_Recclosure = store_thm("Eval_Recclosure",
   ``(!v. a n v ==>
-  Eval ((name,v)::(fname,Recclosure env2 [(fname,name,body)] fname)::env2) body (b (f n))) ==>
-    LOOKUP_VAR fname env (Recclosure env2 [(fname,name,body)] fname) ==>
+  Eval (menv2,cenv2, (name,v)::(fname,Recclosure (menv2,cenv2,env2) [(fname,name,body)] fname)::env2) body (b (f n))) ==>
+    LOOKUP_VAR fname env (Recclosure (menv2,cenv2,env2) [(fname,name,body)] fname) ==>
     Eval env (Var (Short fname)) ((Eq a n --> b) f)``,
   (Eval_Recclosure_ALT |> Q.SPECL [`[(fname,name,body)]`,`fname`]
     |> SIMP_RULE (srw_ss()) [Once find_recfun_def] |> ASSUME_TAC)
@@ -340,9 +323,12 @@ val Eval_Eq_Recclosure = store_thm("Eval_Eq_Recclosure",
     (P f (Recclosure x1 x2 x3) =
      Eval env (Var (Short name)) (P f))``,
   SIMP_TAC std_ss [Eval_Var_SIMP,Eval_def,LOOKUP_VAR_def]
-  \\ SIMP_TAC (srw_ss()) [Once evaluate'_cases]
+  \\ SIMP_TAC (srw_ss()) [Once evaluate_cases]
   \\ REPEAT STRIP_TAC \\ EQ_TAC \\ REPEAT STRIP_TAC
-  \\ FULL_SIMP_TAC std_ss [] \\ METIS_TAC []);
+  \\ PairCases_on `env`
+  \\ FULL_SIMP_TAC std_ss [lookup_var_id_def, LOOKUP_VAR_def]
+  \\ FULL_SIMP_TAC (srw_ss()) []
+  \\ METIS_TAC []);
 
 val Eval_Eq_Fun = store_thm("Eval_Eq_Fun",
   ``Eval env (Fun v x) p ==>
@@ -378,7 +364,10 @@ val Eval_Opn = prove(
   \\ Q.LIST_EXISTS_TAC [`Litv (IntLit n1)`,`Litv (IntLit n2)`]
   \\ FULL_SIMP_TAC (srw_ss()) [do_app_def]
   \\ Cases_on `f` \\ FULL_SIMP_TAC (srw_ss()) []
-  \\ REPEAT (Q.EXISTS_TAC `empty_store`) \\ FULL_SIMP_TAC std_ss []
+  \\ REPEAT (Q.EXISTS_TAC `0,empty_store`) \\ FULL_SIMP_TAC std_ss []
+  \\ Q.EXISTS_TAC `empty_store`
+  \\ Q.EXISTS_TAC `0`
+  \\ SRW_TAC [] []
   \\ ONCE_REWRITE_TAC [evaluate_cases] \\ SIMP_TAC (srw_ss()) []);
 
 local
@@ -403,7 +392,7 @@ val Eval_Opb = prove(
   \\ ONCE_REWRITE_TAC [evaluate_cases] \\ SIMP_TAC (srw_ss()) []
   \\ Q.LIST_EXISTS_TAC [`Litv (IntLit n1)`,`Litv (IntLit n2)`]
   \\ FULL_SIMP_TAC (srw_ss()) [do_app_def]
-  \\ REPEAT (Q.EXISTS_TAC `empty_store`) \\ FULL_SIMP_TAC std_ss []
+  \\ Q.LIST_EXISTS_TAC [`0,empty_store`, `empty_store`, `0`] \\ FULL_SIMP_TAC std_ss []
   \\ ONCE_REWRITE_TAC [evaluate_cases] \\ SIMP_TAC (srw_ss()) []);
 
 local
@@ -442,7 +431,8 @@ val Eval_Num_ABS = store_thm("Eval_Num_ABS",
   SIMP_TAC std_ss [NUM_def]
   \\ `&(Num (ABS i)) = let k = i in if k < 0 then 0 - k else k` by
     (FULL_SIMP_TAC std_ss [LET_DEF] THEN intLib.COOPER_TAC)
-  \\ FULL_SIMP_TAC std_ss [] \\ REPEAT STRIP_TAC \\ MATCH_MP_TAC (GEN_ALL Eval_Let)
+  \\ FULL_SIMP_TAC std_ss [] \\ REPEAT STRIP_TAC
+  \\ PairCases_on `env` \\ MATCH_MP_TAC (GEN_ALL Eval_Let)
   \\ Q.EXISTS_TAC `INT` \\ FULL_SIMP_TAC std_ss [] \\ REPEAT STRIP_TAC
   \\ MATCH_MP_TAC (GEN_ALL (DISCH_ALL th))
   \\ FULL_SIMP_TAC std_ss [Eval_Var_SIMP]);
@@ -507,7 +497,7 @@ val Eval_NUM_SUB = store_thm("Eval_NUM_SUB",
     \\ Cases_on `m<n` \\ FULL_SIMP_TAC std_ss []
     THEN1 (`m - n = 0` by DECIDE_TAC \\ ASM_REWRITE_TAC [])
     \\ FULL_SIMP_TAC std_ss [NOT_LESS,INT_SUB])
-  \\ FULL_SIMP_TAC std_ss [] \\ REPEAT STRIP_TAC \\ MATCH_MP_TAC (GEN_ALL Eval_Let)
+  \\ FULL_SIMP_TAC std_ss [] \\ REPEAT STRIP_TAC \\ PairCases_on `env` \\ MATCH_MP_TAC (GEN_ALL Eval_Let)
   \\ Q.EXISTS_TAC `INT` \\ FULL_SIMP_TAC std_ss [] \\ REPEAT STRIP_TAC
   \\ FULL_SIMP_TAC std_ss [Eval_INT_SUB]
   \\ MATCH_MP_TAC (GEN_ALL (DISCH_ALL th))
@@ -565,7 +555,7 @@ val types_match_def = tDefine "types_match" `
 (* We could change this case to T, or change the semantics to have a type error
  * when equality reaches unequal-length lists *)
 (types_match_list _ _ = F)` (
- WF_REL_TAC `measure (\x. case x of INL (v1,v2) => v_size v1 | INR (vs1,vs2) => v3_size vs1)`);
+ WF_REL_TAC `measure (\x. case x of INL (v1,v2) => v_size v1 | INR (vs1,vs2) => v7_size vs1)`);
 
 val EqualityType_def = Define `
   EqualityType (abs:'a->v->bool) <=>
@@ -617,7 +607,7 @@ val Eval_Equality = store_thm("Eval_Equality",
   \\ Q.LIST_EXISTS_TAC [`res`,`res'`]
   \\ FULL_SIMP_TAC (srw_ss()) [bigClockTheory.do_app_cases]
   \\ Q.EXISTS_TAC `Lit (Bool (res = res'))`
-  \\ REPEAT (Q.EXISTS_TAC `empty_store`) \\ FULL_SIMP_TAC std_ss []
+  \\ Q.LIST_EXISTS_TAC [`0,empty_store`, `empty_store`, `0`] \\ FULL_SIMP_TAC std_ss []
   \\ ONCE_REWRITE_TAC [evaluate_cases]
   \\ FULL_SIMP_TAC (srw_ss()) []
   \\ IMP_RES_TAC do_eq_succeeds
@@ -627,7 +617,7 @@ val Eval_Equality = store_thm("Eval_Equality",
 
 val Decls_def = Define `
   Decls mn (menv1 : envM) cenv1 s1 env1 ds cenv2 s2 env2 =
-    evaluate_decs' mn menv1 cenv1 s1 env1 ds (s2,cenv2, Rval env2)`;
+    evaluate_decs mn (menv1,cenv1,env1) s1 ds (s2,cenv2, Rval env2)`;
 
 val DeclAssum_def = Define `
   DeclAssum ds env = ?s2 cenv2. Decls NONE [] init_envC empty_store [] ds cenv2 s2 env`;
@@ -638,86 +628,75 @@ val Decls_Dtype = store_thm("Decls_Dtype",
       check_dup_ctors mn cenv tds /\ (cenv1 = build_tdefs mn tds) /\
       (env1 = emp) /\ (s1 = s)``,
   SIMP_TAC std_ss [Decls_def]
-  \\ ONCE_REWRITE_TAC [evaluate_decs'_cases] \\ SIMP_TAC (srw_ss()) []
-  \\ ONCE_REWRITE_TAC [evaluate_decs'_cases] \\ SIMP_TAC (srw_ss()) []
-  \\ SIMP_TAC (srw_ss()) [evaluate_dec'_cases, combine_dec_result_def,
-                          merge_def, emp_def]
+  \\ ONCE_REWRITE_TAC [evaluate_decs_cases] \\ SIMP_TAC (srw_ss()) []
+  \\ ONCE_REWRITE_TAC [evaluate_decs_cases] \\ SIMP_TAC (srw_ss()) []
+  \\ SIMP_TAC (srw_ss()) [evaluate_dec_cases, combine_dec_result_def,
+                          merge_def, emp_def, all_env_to_cenv_def]
   \\ METIS_TAC []);
 
 val Decls_Dlet = store_thm("Decls_Dlet",
   ``!mn menv cenv s env v e cenv1 s1 env1.
       Decls mn menv cenv s env [Dlet (Pvar v) e] cenv1 s1 env1 =
       ?x. (cenv1 = emp) /\ (env1 = bind v x emp) /\
-           evaluate' s env e (s1,Rval x)``,
+           evaluate F (menv,cenv,env) (0,s) e ((0,s1),Rval x)``,
   SIMP_TAC std_ss [Decls_def]
-  \\ ONCE_REWRITE_TAC [evaluate_decs'_cases] \\ SIMP_TAC (srw_ss()) []
-  \\ ONCE_REWRITE_TAC [evaluate_decs'_cases] \\ SIMP_TAC (srw_ss()) []
+  \\ ONCE_REWRITE_TAC [evaluate_decs_cases] \\ SIMP_TAC (srw_ss()) []
+  \\ ONCE_REWRITE_TAC [evaluate_decs_cases] \\ SIMP_TAC (srw_ss()) []
   \\ FULL_SIMP_TAC (srw_ss()) [pat_bindings_def,ALL_DISTINCT,MEM,
-       pmatch'_def,bind_def, evaluate_dec'_cases,
+       pmatch_def,bind_def, evaluate_dec_cases,
        combine_dec_result_def, emp_def, merge_def]
-  \\ METIS_TAC []);
+  \\ METIS_TAC [big_unclocked]);
 
 val Decls_Dletrec = store_thm("Decls_Dletrec",
   ``!mn menv cenv s env funs cenv1 s1 env1.
       Decls mn menv cenv s env [Dletrec funs] cenv1 s1 env1 <=>
       ALL_DISTINCT (MAP (\(x,y,z). x) funs) /\
-      (cenv1 = emp) /\ (env1 = build_rec_env funs env emp) /\ (s1 = s)``,
+      (cenv1 = emp) /\ (env1 = build_rec_env funs (menv,cenv,env) emp) /\ (s1 = s)``,
   SIMP_TAC std_ss [Decls_def]
-  \\ ONCE_REWRITE_TAC [evaluate_decs'_cases] \\ SIMP_TAC (srw_ss()) []
-  \\ ONCE_REWRITE_TAC [evaluate_decs'_cases] \\ SIMP_TAC (srw_ss()) []
+  \\ ONCE_REWRITE_TAC [evaluate_decs_cases] \\ SIMP_TAC (srw_ss()) []
+  \\ ONCE_REWRITE_TAC [evaluate_decs_cases] \\ SIMP_TAC (srw_ss()) []
   \\ FULL_SIMP_TAC (srw_ss()) [pat_bindings_def,ALL_DISTINCT,MEM,
-       pmatch_def,bind_def,merge_def, emp_def, evaluate_dec'_cases,
+       pmatch_def,bind_def,merge_def, emp_def, evaluate_dec_cases,
        combine_dec_result_def]
   \\ METIS_TAC []);
 
-val _ = temp_overload_on("has_emp",``\x. FST x = empty_store``)
+val _ = temp_overload_on("has_emp",``\x. SND (FST x) = empty_store``)
 
 val LUPDATE_NIL = prove(
   ``!xs n x. (LUPDATE x n xs = []) = (xs = [])``,
   Cases \\ Cases_on `n` \\ FULL_SIMP_TAC (srw_ss()) [LUPDATE_def]);
 
-val evaluate'_empty_store_lemma = prove(
- ``(!s env e r1.
-      evaluate' s env e r1 ==> has_emp r1 ==> (s = empty_store)) /\
-   (!s env es r1.
-      evaluate_list' s env es r1 ==> has_emp r1 ==> (s = empty_store)) /\
-   (!s env v pes errv r1.
-      evaluate_match' s env v pes errv r1 ==> has_emp r1 ==> (s = empty_store))``,
-  HO_MATCH_MP_TAC evaluate'_ind >> rw [] \\ POP_ASSUM MP_TAC
-  \\ TRY (Cases_on `uop`) \\ TRY (Cases_on `op`)
-  \\ FULL_SIMP_TAC (srw_ss()) [do_uapp_def,do_app_def,LET_DEF,store_alloc_def]
+val evaluate_empty_store_lemma = prove(
+ ``(!ck env s e r1.
+      evaluate ck env s e r1 ==> has_emp r1 ==> (SND s = empty_store)) /\
+   (!ck env s es r1.
+      evaluate_list ck env s es r1 ==> has_emp r1 ==> (SND s = empty_store)) /\
+   (!ck env s v pes errv r1.
+      evaluate_match ck env s v pes errv r1 ==> has_emp r1 ==> (SND s = empty_store))``,
+  HO_MATCH_MP_TAC evaluate_ind >> rw [] \\ POP_ASSUM MP_TAC
+  \\ TRY (Cases_on `uop`) 
+  \\ FULL_SIMP_TAC (srw_ss()) [do_uapp_def,do_app_cases,LET_DEF,store_alloc_def]
   THEN1 (Cases_on `s2`
     \\ FULL_SIMP_TAC (srw_ss()) [store_alloc_def,empty_store_def,APPEND])
   THEN1 (Cases_on `v` \\ FULL_SIMP_TAC (srw_ss()) []
     \\ Cases_on `store_lookup n s2` \\ FULL_SIMP_TAC (srw_ss()) [])
   \\ FULL_SIMP_TAC std_ss [IMP_DISJ_THM]
-  \\ TRY (Cases_on `do_eq v1 v2`) \\ FULL_SIMP_TAC (srw_ss()) []
-  \\ TRY (Cases_on `v1`) \\ FULL_SIMP_TAC (srw_ss()) []
-  \\ TRY (Cases_on `l`) \\ FULL_SIMP_TAC (srw_ss()) []
-  \\ TRY (Cases_on `v2`) \\ FULL_SIMP_TAC (srw_ss()) []
-  \\ TRY (Cases_on `l`) \\ FULL_SIMP_TAC (srw_ss()) []
   \\ SRW_TAC [] []
-  \\ TRY (Cases_on `find_recfun s''' l0` \\ FULL_SIMP_TAC (srw_ss()) [])
-  \\ TRY (Cases_on `x` \\ FULL_SIMP_TAC (srw_ss()) [])
-  \\ TRY (Cases_on `r` \\ FULL_SIMP_TAC (srw_ss()) [])
-  \\ TRY (Cases_on `n < LENGTH s3` \\ FULL_SIMP_TAC (srw_ss()) [])
-  \\ FULL_SIMP_TAC std_ss [store_assign_def,empty_store_def,LUPDATE_NIL]
-  \\ CCONTR_TAC
-  \\ Q.PAT_ASSUM `(if bbb then xxx else zz) = SOME yyy` MP_TAC \\ FULL_SIMP_TAC std_ss []
-  \\ SRW_TAC [] [])
+  \\ FULL_SIMP_TAC std_ss []
+  \\ FULL_SIMP_TAC std_ss [store_assign_def,empty_store_def,LUPDATE_NIL])
   |> SIMP_RULE std_ss [PULL_EXISTS,AND_IMP_INTRO];
 
 val _ = temp_overload_on("has_emp_no_fail",
-  ``\x. (FST x = empty_store:store) /\
+  ``\x. (SND (FST x) = empty_store:store) /\
         ~(SND x = (Rerr Rtype_error):'a result) (*/\
         ~(SND x = (Rerr (Rraise Bind_error)):'a result)*)``)
 
-val sind = IndDefLib.derive_strong_induction(evaluate'_rules,evaluate'_ind);
+val sind = IndDefLib.derive_strong_induction(evaluate_rules,evaluate_ind);
 
 val do_app_empty_store = prove(
   ``!op v1 v2.
       s3 <> empty_store ==>
-      ~(do_app s3 env op v1 v2 = SOME (empty_store,env',e''))``,
+      ~(do_app env s3 op v1 v2 = SOME (env',empty_store,e''))``,
   Cases \\ SIMP_TAC std_ss [do_app_def] \\ SRW_TAC [] []
   \\ BasicProvers.EVERY_CASE_TAC \\ FULL_SIMP_TAC std_ss []
   \\ FULL_SIMP_TAC std_ss [store_assign_def]
@@ -726,8 +705,8 @@ val do_app_empty_store = prove(
 
 val do_app_lemma = prove(
   ``!op.
-      (do_app empty_store env op v1 v2 = SOME (empty_store,env',e'')) ==>
-      !t. do_app t env op v1 v2 = SOME (t,env',e'')``,
+      (do_app env empty_store op v1 v2 = SOME (env',empty_store,e'')) ==>
+      !t. do_app env t op v1 v2 = SOME (env',t,e'')``,
   Cases \\ FULL_SIMP_TAC (srw_ss()) [do_app_def] \\ REPEAT STRIP_TAC
   \\ BasicProvers.EVERY_CASE_TAC \\ FULL_SIMP_TAC std_ss []
   \\ FULL_SIMP_TAC (srw_ss()) [store_assign_def]
@@ -735,41 +714,44 @@ val do_app_lemma = prove(
   \\ TRY (Cases_on `l` \\ FULL_SIMP_TAC (srw_ss()) [])
   \\ FULL_SIMP_TAC (srw_ss()) [empty_store_def]);
 
-val pmatch'_lemma = prove(
-  ``(!(s:store) (p:pat) v env x.
-      (pmatch' empty_store p v env = x) /\ x <> Match_type_error ==>
-      !s. (pmatch' s p v env = x)) /\
-    (!(s:store) (p:pat list) vs env x.
-      (pmatch_list' empty_store p vs env = x) /\ x <> Match_type_error ==>
-      !s. (pmatch_list' s p vs env = x))``,
-  HO_MATCH_MP_TAC pmatch'_ind \\ REPEAT STRIP_TAC
-  \\ FULL_SIMP_TAC std_ss [pmatch'_def]
+val pmatch_lemma = prove(
+  ``(!cenv (s:store) (p:pat) v env x.
+      (pmatch cenv empty_store p v env = x) /\ x <> Match_type_error ==>
+      !s. (pmatch cenv s p v env = x)) /\
+    (!cenv (s:store) (p:pat list) vs env x.
+      (pmatch_list cenv empty_store p vs env = x) /\ x <> Match_type_error ==>
+      !s. (pmatch_list cenv s p vs env = x))``,
+  HO_MATCH_MP_TAC pmatch_ind \\ REPEAT STRIP_TAC
+  \\ FULL_SIMP_TAC std_ss [pmatch_def]
   \\ FULL_SIMP_TAC std_ss [store_lookup_def,empty_store_def,LENGTH]
+  THEN1 (BasicProvers.EVERY_CASE_TAC \\ rw [])
   THEN1 (METIS_TAC [])
-  \\ Cases_on `pmatch' [] p v env`
+  \\ Cases_on `pmatch cenv [] p v env`
   \\ FULL_SIMP_TAC (srw_ss()) []
   \\ Q.PAT_ASSUM `No_match = x` (ASSUME_TAC o GSYM)
   \\ FULL_SIMP_TAC (srw_ss()) []);
 
-val evaluate'_empty_store_IMP_any_store = prove(
- ``(!s env e r1.
-      evaluate' s env e r1 ==> has_emp_no_fail r1 ==>
-      !t. evaluate' t env e (t,SND r1)) /\
-   (!s env es r1.
-      evaluate_list' s env es r1 ==> has_emp_no_fail r1 ==>
-      !t. evaluate_list' t env es (t,SND r1)) /\
-   (!s env v pes errv r1.
-      evaluate_match' s env v pes errv r1 ==> has_emp_no_fail r1 ==>
-      !t. evaluate_match' t env v pes errv (t,SND r1))``,
+val evaluate_empty_store_IMP_any_store = prove(
+ ``(!ck env s e r1.
+      evaluate ck env s e r1 ==> (ck = F) ∧ has_emp_no_fail r1 ==>
+      !t. evaluate ck env t e (t,SND r1)) /\
+   (!ck env s es r1.
+      evaluate_list ck env s es r1 ==> (ck = F) ∧ has_emp_no_fail r1 ==>
+      !t. evaluate_list ck env t es (t,SND r1)) /\
+   (!ck env s v pes errv r1.
+      evaluate_match ck env s v pes errv r1 ==> (ck = F) ∧ has_emp_no_fail r1 ==>
+      !t. evaluate_match ck env t v pes errv (t,SND r1))``,
   HO_MATCH_MP_TAC sind \\ FULL_SIMP_TAC (srw_ss()) [] \\ REPEAT STRIP_TAC
-  \\ ONCE_REWRITE_TAC [evaluate'_cases] \\ FULL_SIMP_TAC (srw_ss()) []
+  \\ ONCE_REWRITE_TAC [evaluate_cases] \\ FULL_SIMP_TAC (srw_ss()) []
   THEN1
    (Cases_on `r1`
-    \\ `s' = empty_store` by IMP_RES_TAC evaluate'_empty_store_lemma
+    \\ `SND s' = empty_store` by IMP_RES_TAC evaluate_empty_store_lemma
     \\ FULL_SIMP_TAC std_ss []
     \\ Cases_on `r` \\ FULL_SIMP_TAC (srw_ss()) [] \\ METIS_TAC [])
   THEN1
-   (Q.LIST_EXISTS_TAC [`v`,`t`] \\ FULL_SIMP_TAC std_ss []
+   METIS_TAC []
+  THEN1
+   (Q.LIST_EXISTS_TAC [`v`,`s2`] \\ FULL_SIMP_TAC std_ss []
     \\ `s2 = empty_store` by ALL_TAC THEN1
      (Cases_on `uop`
       \\ FULL_SIMP_TAC (srw_ss()) [do_uapp_def,LET_DEF,store_alloc_def]
@@ -784,50 +766,53 @@ val evaluate'_empty_store_IMP_any_store = prove(
     \\ FULL_SIMP_TAC (srw_ss()) [do_uapp_def,LET_DEF,
          store_lookup_def,empty_store_def])
   THEN1
-   (`s'' = empty_store` by IMP_RES_TAC evaluate'_empty_store_lemma
+   (`s4 = empty_store` by (IMP_RES_TAC evaluate_empty_store_lemma \\ FULL_SIMP_TAC std_ss [])
     \\ `s3 = empty_store` by METIS_TAC [do_app_empty_store]
     \\ FULL_SIMP_TAC std_ss []
-    \\ `s' = empty_store` by IMP_RES_TAC evaluate'_empty_store_lemma
+    \\ `SND s' = empty_store` by (IMP_RES_TAC evaluate_empty_store_lemma \\ FULL_SIMP_TAC std_ss [])
     \\ FULL_SIMP_TAC std_ss [] \\ IMP_RES_TAC do_app_lemma
-    \\ Cases_on `r1` \\ Cases_on `r` \\ FULL_SIMP_TAC (srw_ss()) [] \\ METIS_TAC [])
-  \\ TRY (`s' = empty_store` by IMP_RES_TAC evaluate'_empty_store_lemma
+    \\ Cases_on `r1` \\ Cases_on `r` \\ FULL_SIMP_TAC (srw_ss()) []
+    \\ METIS_TAC [pair_CASES, FST, SND])
+  \\ TRY (`SND s' = empty_store` by IMP_RES_TAC evaluate_empty_store_lemma
           \\ FULL_SIMP_TAC std_ss [] \\ METIS_TAC [])
   THEN1
-   (`s = empty_store` by IMP_RES_TAC evaluate'_empty_store_lemma
-    \\ FULL_SIMP_TAC std_ss [] \\ IMP_RES_TAC pmatch'_lemma
+   (`s = empty_store` by IMP_RES_TAC evaluate_empty_store_lemma
+    \\ FULL_SIMP_TAC std_ss [] \\ IMP_RES_TAC pmatch_lemma
+    \\ PairCases_on `t`
     \\ FULL_SIMP_TAC (srw_ss()) [])
   THEN1
-   (`s = empty_store` by IMP_RES_TAC evaluate'_empty_store_lemma
-    \\ FULL_SIMP_TAC std_ss [] \\ IMP_RES_TAC pmatch'_lemma
+   (`s = empty_store` by IMP_RES_TAC evaluate_empty_store_lemma
+    \\ FULL_SIMP_TAC std_ss [] \\ IMP_RES_TAC pmatch_lemma
+    \\ PairCases_on `t`
     \\ FULL_SIMP_TAC (srw_ss()) []));
 
-val evaluate'_empty_store_IMP = store_thm("evaluate'_empty_store_IMP",
-  ``evaluate' empty_store env x (empty_store,Rval y) ==>
-    !s. evaluate' s env x (s,Rval y)``,
-  REPEAT STRIP_TAC \\ IMP_RES_TAC evaluate'_empty_store_IMP_any_store
+val evaluate_empty_store_IMP = store_thm("evaluate_empty_store_IMP",
+  ``evaluate F env (c,empty_store) x ((c',empty_store),Rval y) ==>
+    !s. evaluate F env s x (s,Rval y)``,
+  REPEAT STRIP_TAC \\ IMP_RES_TAC evaluate_empty_store_IMP_any_store
   \\ FULL_SIMP_TAC (srw_ss()) []);
 
-val evaluate'_empty_store_EQ = store_thm("evaluate'_empty_store_EQ",
-  ``evaluate' empty_store env x (empty_store,Rval y) =
-    !s. evaluate' s env x (s,Rval y)``,
-  METIS_TAC [evaluate'_empty_store_IMP]);
+val evaluate_empty_store_EQ = store_thm("evaluate_empty_store_EQ",
+  ``evaluate F env (c,empty_store) x ((c,empty_store),Rval y) =
+    !s. evaluate F env s x (s,Rval y)``,
+  METIS_TAC [evaluate_empty_store_IMP]);
 
 val do_app_empty_store = store_thm("do_app_empty_store",
-  ``(do_app s3 env Opapp v1 v2 = SOME (empty_store,env',e3)) <=>
-    (do_app s3 env Opapp v1 v2 = SOME (empty_store,env',e3)) /\ (s3 = empty_store)``,
+  ``(do_app env s3 Opapp v1 v2 = SOME (env',empty_store,e3)) <=>
+    (do_app env s3 Opapp v1 v2 = SOME (env',empty_store,e3)) /\ (s3 = empty_store)``,
   SIMP_TAC (srw_ss()) [do_app_def] \\ Cases_on `v1`
   \\ SIMP_TAC (srw_ss()) [do_app_def] \\ REPEAT BasicProvers.FULL_CASE_TAC
   \\ METIS_TAC []);
 
-val evaluate'_empty_store = store_thm("evaluate'_empty_store",
-  ``evaluate' s2 env xs ((empty_store,Rval ys)) <=>
-    evaluate' s2 env xs ((empty_store,Rval ys)) /\ (s2 = empty_store)``,
+val evaluate_empty_store = store_thm("evaluate_empty_store",
+  ``evaluate F env (c,s2) xs (((c',empty_store),Rval ys)) <=>
+    evaluate F env (c,s2) xs (((c',empty_store),Rval ys)) /\ (s2 = empty_store)``,
   REPEAT STRIP_TAC \\ EQ_TAC \\ REPEAT STRIP_TAC
-  \\ IMP_RES_TAC evaluate'_empty_store_lemma \\ FULL_SIMP_TAC std_ss []);
+  \\ IMP_RES_TAC evaluate_empty_store_lemma \\ FULL_SIMP_TAC std_ss []);
 
-val evaluate_list'_empty_store = prove(
-  ``evaluate_list' s2 env xs (empty_store,Rval ys) ==> (s2 = empty_store)``,
-  REPEAT STRIP_TAC \\ IMP_RES_TAC evaluate'_empty_store_lemma
+val evaluate_list_empty_store = prove(
+  ``evaluate_list F env (c,s2) xs ((c',empty_store),Rval ys) ==> (s2 = empty_store)``,
+  REPEAT STRIP_TAC \\ IMP_RES_TAC evaluate_empty_store_lemma
   \\ FULL_SIMP_TAC (srw_ss()) []);
 
 val combine_dec_result_rval = Q.prove (
@@ -850,12 +835,12 @@ val Decls_APPEND = store_thm("Decls_APPEND",
          Decls mn menv cenv1 s1 env1 ds1 cenv2 s2 env2 /\
          Decls mn menv (merge cenv2 cenv1) s2 (merge env2 env1) ds2 cenv3 s3 env3``,
   Induct_on `ds1` \\ FULL_SIMP_TAC std_ss [APPEND,Decls_def]
-  THEN1 (ONCE_REWRITE_TAC [evaluate_decs'_cases]
+  THEN1 (ONCE_REWRITE_TAC [evaluate_decs_cases]
          \\ SIMP_TAC (srw_ss()) [merge_def, emp_def])
-  \\ SIMP_TAC (srw_ss()) [Once evaluate_decs'_cases]
+  \\ SIMP_TAC (srw_ss()) [Once evaluate_decs_cases]
   \\ FULL_SIMP_TAC std_ss []
   \\ ONCE_REWRITE_TAC [EQ_SYM_EQ]
-  \\ SIMP_TAC (srw_ss()) [Once evaluate_decs'_cases]
+  \\ SIMP_TAC (srw_ss()) [Once evaluate_decs_cases]
   \\ FULL_SIMP_TAC std_ss [PULL_EXISTS]
   \\ rw []
   \\ eq_tac >|
@@ -886,19 +871,19 @@ val Decls_NIL = store_thm("Decls_NIL",
   ``Decls mn menv cenv1 s1 env1 [] cenv2 s2 env2 <=>
       (env2 = emp) /\ (s2 = s1) /\ (cenv2 = emp)``,
   SIMP_TAC std_ss [Decls_def]
-  \\ SIMP_TAC (srw_ss()) [Once evaluate_decs'_cases]
+  \\ SIMP_TAC (srw_ss()) [Once evaluate_decs_cases]
   \\ REPEAT STRIP_TAC \\ EQ_TAC \\ SIMP_TAC std_ss []);
 
 val DeclAssum_Dtype = store_thm("DeclAssum_Dtype",
-  ``(!env. DeclAssum ds env ==> Eval env (Var n) P) ==>
-    !tds. (!env. DeclAssum (SNOC (Dtype tds) ds) env ==> Eval env (Var n) P)``,
+  ``(!env. DeclAssum ds env ==> Eval ([],init_envC,env) (Var n) P) ==>
+    !tds. (!env. DeclAssum (SNOC (Dtype tds) ds) env ==> Eval ([],init_envC,env) (Var n) P)``,
   rw [DeclAssum_def,SNOC_APPEND,Decls_APPEND,Decls_Dtype, merge_def, emp_def]
   \\ METIS_TAC []);
 
 val DeclAssum_Dlet = store_thm("DeclAssum_Dlet",
   ``!ds n P.
-      (!env. DeclAssum ds env ==> Eval env (Var (Short n)) P) ==>
-      !v e. ~(v = n) ==> (!env. DeclAssum (SNOC (Dlet (Pvar v) e) ds) env ==> Eval env (Var (Short n)) P)``,
+      (!env. DeclAssum ds env ==> Eval ([],init_envC,env) (Var (Short n)) P) ==>
+      !v e. ~(v = n) ==> (!env. DeclAssum (SNOC (Dlet (Pvar v) e) ds) env ==> Eval ([],init_envC,env) (Var (Short n)) P)``,
   SIMP_TAC std_ss [DeclAssum_def,SNOC_APPEND,Decls_APPEND,Decls_Dlet]
   \\ REPEAT STRIP_TAC \\ FULL_SIMP_TAC std_ss [APPEND,bind_def,Eval_Var_SIMP, merge_def, emp_def] >>
   rw []
@@ -907,7 +892,7 @@ val DeclAssum_Dlet = store_thm("DeclAssum_Dlet",
 val DeclAssum_Dletrec_LEMMA = prove(
   ``!funs:(varN, varN # exp) env.
       ~MEM n (MAP FST funs) ==>
-      (lookup n (MAP (\(fn,n,e). (fn,Recclosure env2 funs' fn)) funs ++ env2) =
+      (lookup n (MAP (\(fn,n,e). (fn,Recclosure (menv2,cenv2,env2) funs' fn)) funs ++ env2) =
        lookup n (env2:envE))``,
   Induct
   \\ rw []
@@ -927,18 +912,18 @@ val option_CASE_LEMMA = prove(
 
 val DeclAssum_Dletrec = store_thm("DeclAssum_Dletrec",
   ``!ds n P.
-      (!env. DeclAssum ds env ==> Eval env (Var (Short n)) P) ==>
+      (!env. DeclAssum ds env ==> Eval ([],init_envC,env) (Var (Short n)) P) ==>
       !funs. ~(MEM n (MAP FST funs)) ==>
              (!env. DeclAssum (SNOC (Dletrec funs) ds) env ==>
-                    Eval env (Var (Short n)) P)``,
+                    Eval ([],init_envC,env) (Var (Short n)) P)``,
   SIMP_TAC std_ss [DeclAssum_def,SNOC_APPEND,Decls_APPEND,Decls_Dletrec]
   \\ REPEAT STRIP_TAC \\ FULL_SIMP_TAC std_ss [bind_def,Eval_Var_SIMP]
   \\ FULL_SIMP_TAC std_ss [PULL_EXISTS] \\ RES_TAC
   \\ MATCH_MP_TAC Eval_Var_SWAP_ENV
-  \\ Q.EXISTS_TAC `env2` \\ FULL_SIMP_TAC std_ss [merge_def,emp_def,APPEND_NIL]
+  \\ Q.LIST_EXISTS_TAC [`menv2`,`cenv2`,`env2`] \\ FULL_SIMP_TAC std_ss [merge_def,emp_def,APPEND_NIL]
   \\ Q.PAT_ASSUM `n NOTIN set (MAP FST funs)` MP_TAC
   \\ SIMP_TAC std_ss [build_rec_env_def]
-  \\ Q.SPEC_TAC (`Recclosure env2 funs`,`recc`)
+  \\ Q.SPEC_TAC (`Recclosure (menv2,cenv2,env2) funs`,`recc`)
   \\ Q.SPEC_TAC (`funs`,`xs`) \\ Induct
   \\ FULL_SIMP_TAC std_ss [FOLDR,APPEND,FORALL_PROD,MAP,bind_def,
        lookup_def,MEM,bind_def]);
